pcm

concurrency/hack-pcm-shared/MorphismResource.s.dfy
@@ -3,45 +3,40 @@ include "MinimalResourceSpec.s.dfy"
 abstract module MorphismResourceSpec refines MinimalResourceSpec {
   import Base : MinimalResourceSpec
 
-  predicate r(a: Base.R, a': R)
-  ensures r(a, a') ==> Base.Valid(a) && Valid(a')
+  type M' = M
 
-  lemma init_unit(a': R)
+  predicate r(a: Base.M, a': M')
+
+  lemma init_unit(a': M')
   requires Init(a')
   ensures r(Base.unit(), a')
 
-  lemma morphism_additive(a: Base.R, b: Base.R, a': R, b': R)
-  requires Base.Valid(a)
-  requires Base.Valid(b)
-  requires Valid(a')
-  requires Valid(b')
+  lemma morphism_additive(a: Base.M, b: Base.M, a': M', b': M')
   requires r(a, a')
   requires r(b, b')
-  requires Base.Valid(Base.add(a, b))
-  ensures r(Base.add(a, b), add(a',b'))
+  requires Base.add_defined(a, b)
+  ensures add_defined(a', b')
+  ensures r(Base.add(a, b), add(a', b'))
 
-  lemma morphism_subtractive(a: Base.R, b: Base.R, a': R, b': R)
-  requires Base.Valid(a)
-  requires Base.Valid(b)
-  requires Valid(a')
-  requires Valid(b')
+  lemma morphism_subtractive(a: Base.M, b: Base.M, a': M', b': M')
   requires r(a, a')
-  requires Base.Valid(Base.add(a, b))
-  requires r(Base.add(a, b), add(a',b'))
+  requires Base.add_defined(a, b)
+  requires add_defined(a', b')
+  requires r(Base.add(a, b), add(a', b'))
   ensures r(b, b')
 
-  least predicate transition_closure(a: Base.R, b: Base.R)
+  least predicate transition_closure(a: Base.M, b: Base.M)
   {
     a == b || (exists c :: transition_closure(a, c) && Base.transition(c, b))
   }
 
-  lemma self_transition(a: Base.R, b: Base.R, a': R)
+  lemma self_transition(a: Base.M, b: Base.M, a': M')
   requires r(a, a')
   requires r(b, a')
   ensures transition_closure(a, b)
 
-  lemma transition_transition(a: Base.R, a': R, b': R)
-  returns (b: Base.R)
+  lemma transition_transition(a: Base.M, a': M', b': M')
+  returns (b: Base.M)
   requires r(a, a')
   requires transition(a', b')
   ensures r(b, b')
@@ -51,18 +46,18 @@ abstract module MorphismResourceSpec refines MinimalResourceSpec {
    * Actions
    */
 
-  function method {:extern} translate_to(linear a: Base.R, ghost expected_out: R)
-      : (linear out: R)
+  function method {:extern} translate_to(linear a: Base.M, ghost expected_out: M')
+      : (linear out: M')
   requires r(a, expected_out)
   ensures out == expected_out
 
-  function method {:extern} translate_from(linear a': R, ghost expected_out: Base.R)
-      : (linear out: Base.R)
+  function method {:extern} translate_from(linear a': M', ghost expected_out: Base.M)
+      : (linear out: Base.M)
   requires r(expected_out, a')
   ensures out == expected_out
 
-  function method {:extern} translate_shared(shared s': R, ghost expected_out: Base.R)
-      : (linear s: Base.R)
+  function method {:extern} translate_shared(shared s': M', ghost expected_out: Base.M)
+      : (linear s: Base.M)
   requires forall a, a' :: r(a, a') && W(a', s') ==> Base.W(a, expected_out)
   ensures s == expected_out
 }
